Prove compile_correct except while case

pancake/pan_simpScript.sml
@@ -9,32 +9,64 @@ val _ = set_grammar_ancestry ["panLang","backend_common"];
 
 val _ = patternMatchesLib.ENABLE_PMATCH_CASES();
 
-Definition skip_seq_def:
-   skip_seq p q =
+Definition SmartSeq_def[simp]:
+   SmartSeq p q =
     if p = Skip then q else Seq p q
 End
 
 Definition seq_assoc_def:
   (seq_assoc p Skip = p) /\
   (seq_assoc p (Dec v e q) =
-    skip_seq p (Dec v e (seq_assoc Skip q))) /\
+    SmartSeq p (Dec v e (seq_assoc Skip q))) /\
   (seq_assoc p (Seq q r) = seq_assoc (seq_assoc p q) r) /\
   (seq_assoc p (If e q r) =
-    skip_seq p (If e (seq_assoc Skip q) (seq_assoc Skip r))) /\
+    SmartSeq p (If e (seq_assoc Skip q) (seq_assoc Skip r))) /\
   (seq_assoc p (While e q) =
-    skip_seq p (While e (seq_assoc Skip q))) /\
+    SmartSeq p (While e (seq_assoc Skip q))) /\
   (seq_assoc p (Call rtyp name args) =
-    skip_seq p (Call
+    SmartSeq p (Call
                  (dtcase rtyp of
                    | Tail => Tail
                    | Ret v => Ret v
                    | Handle v v' s q => Handle v v' s (seq_assoc Skip q))
                 name args)) /\
-  (seq_assoc p others = skip_seq p others)
+  (seq_assoc p others = SmartSeq p others)
 End
 
-(* we need to have a recusive def *)
+Theorem seq_assoc_pmatch:
+  !p prog.
+  seq_assoc p prog =
+  case prog of
+  | Skip => p
+  | (Dec v e q) => SmartSeq p (Dec v e (seq_assoc Skip q))
+  | (Seq q r) => seq_assoc (seq_assoc p q) r
+  | (If e q r) =>
+     SmartSeq p (If e (seq_assoc Skip q) (seq_assoc Skip r))
+  | (While e q) =>
+     SmartSeq p (While e (seq_assoc Skip q))
+  | (Call rtyp name args) =>
+     SmartSeq p (Call
+                 (dtcase rtyp of
+                   | Tail => Tail
+                   | Ret v => Ret v
+                   | Handle v v' s q => Handle v v' s (seq_assoc Skip q))
+                name args)
+  | other => SmartSeq p other
+Proof
+  rpt strip_tac >>
+  CONV_TAC(RAND_CONV patternMatchesLib.PMATCH_ELIM_CONV) >>
+  every_case_tac >> fs[seq_assoc_def]
+QED
 
+Definition retcall_ret_to_tail_def:
+  retcall_ret_to_tail prog =
+   dtcase prog of
+    | Seq (RetCall v trgt args) (Return (Var v')) =>
+      if v = v' then TailCall trgt args else Seq (RetCall v trgt args) (Return (Var v'))
+    | other => other
+End
+
+(*
 Definition retcall_ret_to_tail_def:
   retcall_ret_to_tail prog =
    case prog of
@@ -42,6 +74,21 @@ Definition retcall_ret_to_tail_def:
       TailCall trgt args
     | other => other
 End
+
+
+Theorem retcall_ret_to_tail_pmatch:
+  !prog.
+  retcall_ret_to_tail prog =
+  case prog of
+  | Seq (RetCall v trgt args) (Return (Var v)) =>
+      TailCall trgt args
+  | other => other
+Proof
+  rpt strip_tac >>
+  CONV_TAC(RAND_CONV patternMatchesLib.PMATCH_ELIM_CONV) >>
+  every_case_tac >> fs[seq_assoc_def]
+QED
+*)
 
 Definition retcall_elim_def:
   (retcall_elim Skip = Skip) /\
@@ -58,6 +105,32 @@ Definition retcall_elim_def:
     name args) /\
   (retcall_elim others = others)
 End
+
+
+Theorem retcall_elim_pmatch:
+  !p.
+  retcall_elim p =
+  case p of
+  | Skip => Skip
+  | (Dec v e q) => Dec v e (retcall_elim q)
+  | (Seq q r) => retcall_ret_to_tail (Seq (retcall_elim q) (retcall_elim r))
+  | (If e q r) =>
+     If e (retcall_elim q) (retcall_elim r)
+  | (While e q) =>
+     While e (retcall_elim q)
+  | (Call rtyp name args) =>
+     Call
+     (dtcase rtyp of
+       | Tail => Tail
+       | Ret v => Ret v
+       | Handle v v' s q => Handle v v' s (retcall_elim q))
+    name args
+  | other => other
+Proof
+  rpt strip_tac >>
+  CONV_TAC(RAND_CONV patternMatchesLib.PMATCH_ELIM_CONV) >>
+  every_case_tac >> fs[retcall_elim_def]
+QED
 
 
 Definition compile_prog_def:
