pancake/proofs/pan_simpProofScript.sml
@@ -1,0 +1,194 @@
+(*
+  Correctness proof for pan_simp
+*)
+
+open preamble panLangTheory pan_simpTheory panSemTheory
+
+val _ = new_theory "pan_simpProof";
+
+val _ = set_grammar_ancestry ["panLang", "pan_simp", "panSem"];
+
+val s = ``s:('a,'ffi) panSem$state``
+
+Theorem evaluate_SmartSeq:
+  evaluate (SmartSeq p q,s) = evaluate (Seq p q,^s)
+Proof
+  rw [SmartSeq_def, evaluate_def]
+QED
+
+Theorem evaluate_seq_skip:
+   !p s. evaluate (Seq p Skip,s) = evaluate (p,^s)
+Proof
+  Induct >> fs [Once evaluate_def] >> rw [] >>
+  rpt (pairarg_tac >> fs [] >> rw [evaluate_def] >> fs [])
+QED
+
+Theorem evaluate_skip_seq:
+  evaluate (Seq Skip p,s) = evaluate (p,^s)
+Proof
+  fs [evaluate_def]
+QED
+
+Theorem evaluate_seq_assoc:
+  !p q s. evaluate (seq_assoc p q,s) = evaluate (Seq p q,^s)
+Proof
+  ho_match_mp_tac seq_assoc_ind >> rw [] >>
+  fs [evaluate_seq_skip, seq_assoc_def] >>
+  TRY (rename1 ‘While’ >> cheat) >>
+  fs [evaluate_def] >> rpt (pairarg_tac >> fs [] >> rw [] >> fs []) >>
+  every_case_tac >> fs [] >> rveq  >> fs [evaluate_skip_seq, evaluate_def]
+QED
+
+
+Theorem eval_set_var_lookup_eq:
+  eval (s with locals := lcs |+ (v,value)) (Var v) =
+  SOME value
+Proof
+  rw [eval_def, FLOOKUP_UPDATE]
+QED
+
+Theorem evaluate_retcall_ret_to_tail_eq:
+  !p s.
+   FST (evaluate (p,s)) <> SOME Error ==>
+   evaluate (retcall_ret_to_tail p,s) = evaluate (p,s)
+Proof
+  rw [retcall_ret_to_tail_def] >>
+  every_case_tac >> fs [] >> rveq >>
+  fs [evaluate_def] >>
+  pairarg_tac >> fs [] >>
+  every_case_tac >> fs [] >> rveq >>
+  TRY (metis_tac [] >> NO_TAC) >>
+  fs [empty_locals_def, set_var_def] >>
+  fs [eval_set_var_lookup_eq]
+QED
+
+
+Theorem evaluate_seq_no_error_fst:
+  FST (evaluate (Seq p p',s)) ≠ SOME Error ==>
+  FST (evaluate (p,s)) ≠ SOME Error
+Proof
+  rw [evaluate_def] >>
+  rpt (pairarg_tac >> fs []) >>
+  every_case_tac >> fs[]
+QED
+
+val goal =
+  ``λ(prog, s).
+    FST (evaluate (prog,s)) <> SOME Error ==>
+    evaluate (retcall_elim prog, s) = evaluate (prog,s)``
+
+local
+  val ind_thm = panSemTheory.evaluate_ind
+    |> ISPEC goal
+    |> CONV_RULE (DEPTH_CONV PairRules.PBETA_CONV) |> REWRITE_RULE [];
+  fun list_dest_conj tm = if not (is_conj tm) then [tm] else let
+    val (c1,c2) = dest_conj tm in list_dest_conj c1 @ list_dest_conj c2 end
+  val ind_goals = ind_thm |> concl |> dest_imp |> fst |> list_dest_conj
+in
+  fun get_goal s = first (can (find_term (can (match_term (Term [QUOTE s]))))) ind_goals
+  fun retcall_elim_tm () = ind_thm |> concl |> rand
+  fun the_ind_thm () = ind_thm
+end
+
+
+Theorem retcall_elim_dec:
+  ^(get_goal "panLang$Dec")
+Proof
+  rw [retcall_elim_def] >>
+  fs [evaluate_def] >>
+  TOP_CASE_TAC >> fs [] >>
+  rpt (pairarg_tac >> fs [] >> rveq)
+QED
+
+
+Theorem retcall_elim_seq:
+  ^(get_goal "panLang$Seq")
+Proof
+  rw [retcall_elim_def] >>
+  qmatch_goalsub_abbrev_tac ‘retcall_ret_to_tail sprog’ >>
+  ‘evaluate (retcall_ret_to_tail sprog,s) = evaluate (sprog,s)’ by (
+    ho_match_mp_tac evaluate_retcall_ret_to_tail_eq >>
+    unabbrev_all_tac >>
+    imp_res_tac evaluate_seq_no_error_fst >> fs [] >>
+    fs [evaluate_def] >>
+    pairarg_tac >> fs [] >>
+    TOP_CASE_TAC >> fs []) >>
+  fs [] >> pop_assum kall_tac >>
+  unabbrev_all_tac >>
+  rw [evaluate_def] >>
+  rpt (pairarg_tac >> fs []) >>
+  every_case_tac >> fs [] >> rveq >>
+  fs [evaluate_def]
+QED
+
+
+Theorem retcall_elim_if:
+  ^(get_goal "panLang$If")
+Proof
+  rw [retcall_elim_def] >>
+  fs [evaluate_def] >>
+  every_case_tac >> fs [] >>
+  rpt (pairarg_tac >> fs [] >> rveq)
+QED
+
+
+Theorem retcall_elim_while:
+  ^(get_goal "panLang$While")
+Proof
+ cheat
+QED
+
+
+Theorem retcall_elim_call:
+  ^(get_goal "panLang$Call")
+Proof
+  rw [retcall_elim_def] >>
+  fs [evaluate_def] >>
+  every_case_tac >> fs []
+QED
+
+
+Theorem retcall_elim_others:
+  ^(get_goal "panLang$Skip") /\
+  ^(get_goal "panLang$Assign") /\
+  ^(get_goal "panLang$Store") /\
+  ^(get_goal "panLang$StoreByte") /\
+  ^(get_goal "panLang$Break") /\
+  ^(get_goal "panLang$Continue") /\
+  ^(get_goal "panLang$ExtCall") /\
+  ^(get_goal "panLang$Raise") /\
+  ^(get_goal "panLang$Return") /\
+  ^(get_goal "panLang$Tick")
+Proof
+  rw [retcall_elim_def]
+QED
+
+Theorem retcall_elim_correct:
+  ^(retcall_elim_tm())
+Proof
+  match_mp_tac (the_ind_thm()) >>
+  EVERY (map strip_assume_tac [retcall_elim_dec, retcall_elim_seq,
+         retcall_elim_if, retcall_elim_while, retcall_elim_call,
+         retcall_elim_others]) >>
+  asm_rewrite_tac [] >> rw [] >> rpt (pop_assum kall_tac)
+QED
+
+Theorem foo:
+  FST (evaluate (p,s)) ≠ SOME Error ==>
+      FST (evaluate ((seq_assoc Skip p),s)) ≠ SOME Error
+Proof
+  rw [evaluate_seq_assoc] >>
+  rw [evaluate_def]
+QED
+
+Theorem compile_correct:
+  FST (evaluate (p,s)) <> SOME Error ==>
+    evaluate (compile_prog p, s) = evaluate (p,s)
+Proof
+  rw [compile_prog_def] >>
+  dxrule foo >> strip_tac >>
+  imp_res_tac retcall_elim_correct >> fs [] >>
+  rw [evaluate_seq_assoc, evaluate_def]
+QED
+
+val _ = export_theory();
